- fix a bug in rule - remove unused defs - more simple cases in completeness

proof/old_system/uni/def_ott.v
@@ -1486,9 +1486,7 @@ Inductive a_mono_typ : aenv -> typ -> Prop :=    (* defn a_mono_typ *)
  | a_mono_typ__tvar : forall (aE:aenv) (X:typvar),
       binds ( X )  ( abind_tvar_empty ) ( aE )  ->
      a_mono_typ aE (typ_var_f X)
- | a_mono_typ__etvar : forall (aE:aenv) (X:typvar) (A B:typ),
-     a_wf_typ aE A ->
-     a_wf_typ aE B ->
+ | a_mono_typ__etvar : forall (aE:aenv) (X:typvar),
       binds ( X )  ( abind_etvar_empty ) ( aE )  ->
      a_mono_typ aE (typ_var_f X)
  | a_mono_typ__arrow : forall (aE:aenv) (A1 A2:typ),
